Some layout algebra

src/lib/data/Kuiper.Index.fst
@@ -60,6 +60,56 @@ let rec modulo_i (#n:nat) (i : natlt n) (d : idesc n) : idesc (n-1) =
     | 0 -> ts
     | i -> ICons t (modulo_i (i-1) ts)
 
+(* Insert a dimension. Note the n+1, one can insert at the very end. *)
+let rec insert_i (#n:nat) (i : natlt (n+1)) (k : nat) (d : idesc n) : idesc (n+1) =
+  match i with
+  | 0 -> ICons k d
+  | i -> ICons (d @! 0) (insert_i (i-1) k (modulo_i 0 d))
+
+(* Silence warning about using '-' in patterns. It's in an implicit,
+not much to do, and it works. *)
+#push-options "--warn_error -271"
+let rec insert_modulo (#n:nat) (i : natlt n) (d : idesc n)
+  : Lemma (insert_i #(n-1) i (d @! i) (modulo_i i d) == d)
+          [SMTPat (insert_i #(n-1) i (d @! i) (modulo_i i d))]
+  = match d with
+    | INil -> ()
+    | ICons t ts ->
+      match i with
+      | 0 -> ()
+      | i -> insert_modulo (i-1) ts
+
+let rec modulo_insert (#n:nat) (i : natlt (n+1)) (k : nat) (d : idesc n)
+  : Lemma (ensures modulo_i i (insert_i i k d) == d)
+          [SMTPat (modulo_i i (insert_i i k d))]
+  = match i with
+    | 0 -> ()
+    | i ->
+      match d with
+      | INil -> assert false
+      | ICons t ts -> modulo_insert (i-1) k ts
+
+let rec modulo_size_lemma (#n:nat) (i : natlt n) (d : idesc n)
+  : Lemma (sizeof (modulo_i i d) * (d @! i) == sizeof d)
+          [SMTPat (sizeof (modulo_i i d)); SMTPat (sizeof d)]
+  = match d with
+    | INil -> ()
+    | ICons t ts ->
+      match i with
+      | 0 -> ()
+      | i -> modulo_size_lemma (i-1) ts
+
+let rec insert_size_lemma (#n:nat) (i : natlt (n+1)) (k : nat) (d : idesc n)
+  : Lemma (sizeof (insert_i i k d) == sizeof d * k)
+          [SMTPat (sizeof (insert_i i k d)); SMTPat (sizeof d)]
+  = match i with
+    | 0 -> ()
+    | i ->
+      match d with
+      | INil -> assert false
+      | ICons t ts -> insert_size_lemma (i-1) k ts
+#pop-options
+
 let abs_bring_forward_bij (#n:nat) (i : natlt n) (d : idesc n)
   : (abs d =~ natlt (d @! i) & abs (modulo_i i d))
   = magic()
