src/lib/data/Kuiper.TensorLayout.fsti
@@ -1,0 +1,118 @@
+module Kuiper.TensorLayout
+
+open Kuiper
+open Kuiper.Injection
+open Kuiper.Index
+open Kuiper.Chest
+open FStar.Tactics.Typeclasses { no_method }
+module V = Kuiper.View
+module SZ = Kuiper.SizeT
+module T = FStar.Tactics.V2
+
+[@@erasable]
+noeq
+type tlayout (#r : erased nat) (d : idesc r) = {
+  (* Underlying length of base array (Kuiper.Array) *)
+  ulen : nat;
+  (* Injection from (abstract) index space into base array. *)
+  imap : abs d @~> natlt ulen;
+}
+
+(* Alias for .ulen *)
+let tlayout_size (#d : idesc 'r) (l : tlayout d) : GTot nat = l.ulen
+
+inline_for_extraction
+class ctlayout (#r : erased nat) (#d : idesc r) (l : tlayout d) = {
+  [@@@no_method]
+  culen : (x : SZ.t { SZ.v x == l.ulen });
+
+  [@@@no_method]
+  cimap : i:conc d -> r:SZ.t{SZ.v r == l.imap.f ((abs_conc_bij d).gg i)};
+}
+
+let tensor_aview (et : Type) (#r : nat) (#d : idesc r) (l : tlayout d)
+  : V.aview et (chest d et)
+  = {
+      iview = {
+        len = l.ulen;
+        ait = abs d;
+        step = { imap = l.imap; };
+      };
+      ctn = solve;
+    }
+
+(* First attempt at constructing tensor layouts. *)
+
+let f_grouped_by (#n:nat)
+  (#d : idesc n)
+  (i : natlt n)
+  (sub : abs (modulo_i i d) @~> natlt (sizeof (modulo_i i d)))
+  : (abs d @~> natlt (sizeof d))
+  =
+  mk_injection #(abs d) #(natlt (sizeof d))
+    (fun (idx : abs d) ->
+      let maj, min = (abs_bring_forward_bij i d).ff idx in
+      let sub_i : natlt (sizeof (modulo_i i d)) = sub.f min in
+      let offset = maj * sizeof (modulo_i i d) in
+      offset + sub_i)
+    (fun _ _ -> ())
+
+let lunit : (abs INil @~> natlt 1) =
+  mk_injection #(abs INil) #(natlt 1) (fun () -> 0) ez
+
+let row_major (m n : nat) : (abs (ICons m <| ICons n INil) @~> natlt (m*n)) =
+  f_grouped_by #2 #(ICons m <| ICons n INil) 0 <|
+  f_grouped_by #1 #(ICons n INil)            0 <|
+  lunit
+
+let col_major (m n : nat) : (abs (ICons m <| ICons n INil) @~> natlt (m*n)) =
+  f_grouped_by #2 #(ICons m <| ICons n INil) 1 <|
+  f_grouped_by #1 #(ICons m INil)            0 <|
+  lunit
+
+let batched_row_major (r m n : nat) :
+  (abs (ICons r <| ICons m <| ICons n INil) @~> natlt (r*m*n))
+=
+  f_grouped_by #_ #(ICons r <| ICons m <| ICons n INil) 0 <|
+  f_grouped_by #_ #(ICons m <| ICons n INil)            0 <|
+  f_grouped_by #_ #(ICons n INil)                       0 <|
+  lunit
+
+(* Second attempt at constructing tensor layouts. *)
+
+let g_grouped_by (#n:nat)
+  (i : natlt (n+1))
+  (k : nat)
+  (#d : idesc n)
+  (sub : abs d @~> natlt (sizeof d))
+  : (abs (insert_i i k d) @~> natlt (sizeof (insert_i i k d)))
+  =
+  mk_injection #(abs (insert_i i k d)) #(natlt (sizeof (insert_i i k d)))
+    (fun (idx : abs (insert_i i k d)) ->
+      modulo_insert i k d;
+      let maj, min = (abs_bring_forward_bij i (insert_i i k d)).ff idx in
+      let sub_i : natlt (sizeof d) = sub.f min in
+      let offset = maj * sizeof d in
+      offset + sub_i)
+    (fun idx1 idx2 ->
+      let maj1, min1 = (abs_bring_forward_bij i (insert_i i k d)).ff idx1 in
+      let maj2, min2 = (abs_bring_forward_bij i (insert_i i k d)).ff idx2 in
+      ())
+
+let row_major' (m n : nat) : (abs (ICons m <| ICons n INil) @~> natlt (m*n)) =
+  g_grouped_by 0 m  <|
+  g_grouped_by 0 n  <|
+  lunit
+
+let col_major' (m n : nat) : (abs (ICons m <| ICons n INil) @~> natlt (m*n)) =
+  g_grouped_by 1 n <|
+  g_grouped_by 0 m <|
+  lunit
+
+let batched_row_major' (r m n : nat) :
+  (abs (ICons r <| ICons m <| ICons n INil) @~> natlt (r*m*n))
+=
+  g_grouped_by 0 r <|
+  g_grouped_by 0 m <|
+  g_grouped_by 0 n <|
+  lunit
